src/ExternUtils.fst
@@ -1,0 +1,109 @@
+module ExternUtils
+
+module G = FStar.Ghost
+module U8 = FStar.UInt8
+module U32 = FStar.UInt32
+module U64 = FStar.UInt64
+module US = FStar.SizeT
+
+open Steel.Effect.Atomic
+open Steel.Effect
+open Steel.Reference
+module A = Steel.Array
+
+open Config
+open Utils2
+
+assume val ffs64 (x: U64.t) (bound: G.erased U32.t)
+  : Pure U32.t
+  (requires
+    U32.v (G.reveal bound) <= 64 /\
+    (exists (k:nat{k < U32.v (G.reveal bound)}). nth_is_zero x (U32.uint_to_t k)))
+  (ensures fun r ->
+    U32.v r < U32.v (G.reveal bound) /\
+    nth_is_zero x r /\
+    (forall (k:nat{k < U64.n /\ nth_is_zero x (U32.uint_to_t k)}).
+      U32.v r <= k
+    )
+  )
+
+assume val apply_zeroing_u8
+  (ptr: array U8.t)
+  (n: US.t)
+  : Steel unit
+  (A.varray ptr)
+  (fun _ -> A.varray ptr)
+  (requires fun h0 ->
+    A.length ptr >= US.v n
+  )
+  (ensures fun h0 _ h1 ->
+    A.length ptr >= US.v n /\
+    zf_u8 (Seq.slice (A.asel ptr h1) 0 (US.v n))
+  )
+
+let apply_zeroing_u8_cond
+  (ptr: array U8.t)
+  (n: US.t)
+  : Steel unit
+  (A.varray ptr)
+  (fun _ -> A.varray ptr)
+  (requires fun h0 ->
+    A.length ptr >= US.v n
+  )
+  (ensures fun h0 _ h1 ->
+    A.length ptr >= US.v n /\
+    (not enable_zeroing_free ==>
+      A.asel ptr h1 == A.asel ptr h0
+    ) /\
+    (enable_zeroing_free ==>
+      zf_u8 (Seq.slice (A.asel ptr h1) 0 (US.v n))
+    )
+  )
+  =
+  if enable_zeroing_free then (
+    apply_zeroing_u8 ptr n
+  ) else (
+    return ()
+  )
+
+assume val check_zeroing_u8
+  (ptr: array U8.t)
+  (n: US.t)
+  : Steel bool
+  (A.varray ptr)
+  (fun _ -> A.varray ptr)
+  (requires fun _ ->
+    A.length ptr >= US.v n
+  )
+  (ensures fun h0 b h1 ->
+    A.length ptr >= US.v n /\
+    (b ==> zf_u8 (Seq.slice (A.asel ptr h1) 0 (US.v n)))
+  )
+
+assume val memcpy_u8
+  (dest src: array U8.t) (n: US.t)
+  : Steel (array U8.t)
+  (A.varray dest `star` A.varray src)
+  (fun _ -> A.varray dest `star` A.varray src)
+  (requires fun _ ->
+    A.length dest >= US.v n /\
+    A.length src >= US.v n
+  )
+  (ensures fun h0 r h1 ->
+    A.length dest >= US.v n /\
+    A.length src >= US.v n /\
+    Seq.slice (A.asel dest h1) 0 (US.v n)
+    ==
+    Seq.slice (A.asel src h0) 0 (US.v n) /\
+    A.asel src h1 == A.asel src h0
+  )
+
+open FStar.Mul
+
+assume val builtin_mul_overflow(x y: US.t)
+  : Pure US.t
+  (requires True)
+  (ensures fun r ->
+    US.fits (US.v x * US.v y) /\
+    US.v r == US.v x * US.v y
+  )
