src/Guards2.fst
@@ -1,0 +1,13 @@
+module Guards2
+
+let guard_slab size_class arr
+  = if enable_guard_pages then trap_array arr else A.varray arr
+
+let mmap_trap_guard size_class arr len =
+  if enable_guard_pages then (
+    mmap_strict_trap arr len;
+    change_equal_slprop (trap_array arr) (guard_slab size_class arr)
+  ) else (
+    noop ();
+    change_equal_slprop (A.varray arr) (guard_slab size_class arr)
+  )
