src/MemoryTrap.fsti
@@ -1,7 +1,6 @@
- module MemoryTrap
+module MemoryTrap
 
 open Utils2
-open SlotsAlloc
 
 open Steel.Effect.Atomic
 open Steel.Effect
@@ -28,39 +27,67 @@ val trap_array (arr: array U8.t) : vprop
 /// Introduction function for the abstract `trap_array`
 /// predicate above. Under the hood, this function will
 /// be implemented in C as a mmap(PROT_NONE)
+// assume val
 val mmap_strict_trap
   (arr: array U8.t)
-  (len: US.t{US.v len == A.length arr /\ US.v len > 0})
-  : SteelT unit
+  (len: US.t)
+  : Steel unit
   (A.varray arr)
   (fun _ -> trap_array arr)
+  (requires fun _ ->
+    A.length arr == US.v len /\
+    US.v len % U32.v page_size == 0 /\
+    US.v len > 0
+  )
+  (ensures fun _ _ _ -> True)
 ///
 /// Introduction function for the abstract `trap_array`
 /// predicate above. Under the hood, this function will
 /// be implemented in C as a madvise(MADV_DONTNEED)
+// assume val
 val mmap_trap
   (arr: array U8.t)
-  (len: US.t{US.v len == A.length arr /\ US.v len > 0})
-  : SteelT unit
+  (len: US.t)
+  : Steel unit
   (A.varray arr)
   (fun _ -> trap_array arr)
+  (requires fun _ ->
+    A.length arr == US.v len /\
+    US.v len % U32.v page_size == 0 /\
+    US.v len > 0
+  )
+  (ensures fun _ _ _ -> True)
 
 /// Elimination function for the abstract `trap_array`
 /// predicate above. Under the hood, this function will
 /// be implemented in C as a mmap(PROT_READ|PROT_WRITE)
+// assume val
 val mmap_strict_untrap
   (arr: array U8.t)
-  (len: US.t{US.v len == A.length arr /\ US.v len > 0})
-  : SteelT unit
+  (len: US.t)
+  : Steel unit
   (trap_array arr)
   (fun _ -> A.varray arr)
+  (requires fun _ ->
+    A.length arr == US.v len /\
+    US.v len % U32.v page_size == 0 /\
+    US.v len > 0
+  )
+  (ensures fun _ _ _ -> True)
 
 /// Elimination function for the abstract `trap_array`
 /// predicate above. Under the hood, this function will
 /// be implemented in C as a noop.
+// assume val
 val mmap_untrap
   (arr: array U8.t)
-  (len: US.t{US.v len == A.length arr /\ US.v len > 0})
-  : SteelT unit
+  (len: US.t)
+  : Steel unit
   (trap_array arr)
   (fun _ -> A.varray arr)
+  (requires fun _ ->
+    A.length arr == US.v len /\
+    US.v len % U32.v page_size == 0 /\
+    US.v len > 0
+  )
+  (ensures fun _ _ _ -> True)
