src/Quarantine.fst
@@ -6,6 +6,7 @@ let quarantine_slab arr =
   else A.varray arr
 
 let mmap_trap_quarantine arr len =
+  ();
   if enable_quarantine_trap then (
     if enable_quarantine_strict_trap then (
       mmap_strict_trap arr len
