src/Quarantine2.fst
@@ -1,0 +1,40 @@
+module Quarantine2
+
+let quarantine_slab size_class arr =
+  if enable_quarantine_trap
+  then trap_array arr
+  else A.varray arr
+
+let mmap_trap_quarantine size_class arr len =
+  if enable_quarantine_trap then (
+    if enable_quarantine_strict_trap then (
+      mmap_strict_trap arr len
+    ) else (
+      mmap_trap arr len
+    );
+    change_equal_slprop
+      (trap_array arr)
+      (quarantine_slab size_class arr)
+  ) else (
+    noop ();
+    change_equal_slprop
+      (A.varray arr)
+      (quarantine_slab size_class arr)
+  )
+
+let mmap_untrap_quarantine size_class arr len =
+  if enable_quarantine_trap then (
+    change_equal_slprop
+      (quarantine_slab size_class arr)
+      (trap_array arr);
+    if enable_quarantine_strict_trap then (
+      mmap_strict_untrap arr len
+    ) else (
+      mmap_untrap arr len
+    )
+  ) else (
+    noop ();
+    change_equal_slprop
+      (quarantine_slab size_class arr)
+      (A.varray arr)
+  )
