src/Utils2.fsti
@@ -129,19 +129,6 @@ let nth_is_zero (x: U64.t) (pos: U32.t{U32.v pos < 64})
   = FU.nth (U64.v x) (U64.n - U32.v pos - 1) = false
 
 module G = FStar.Ghost
-// CAUTION: assume val, no implementation
-val ffs64 (x: U64.t) (bound: G.erased U32.t)
-  : Pure U32.t
-  (requires
-    U32.v (G.reveal bound) <= 64 /\
-    (exists (k:nat{k < U32.v (G.reveal bound)}). nth_is_zero x (U32.uint_to_t k)))
-  (ensures fun r ->
-    U32.v r < U32.v (G.reveal bound) /\
-    nth_is_zero x r /\
-    (forall (k:nat{k < U64.n /\ nth_is_zero x (U32.uint_to_t k)}).
-      U32.v r <= k
-    )
-  )
 
 let max64_lemma_aux (i:nat{i < 64})
   : Lemma
